src/proofs/ElimLet/BindingProofs.v
@@ -2,6 +2,7 @@
 Require Import TermFuncs StateHoareMonad StateInvarPres.
 
 Local Open Scope Z_scope.
+Set Bullet Behavior "Strict Subproofs".
 
 (*Part 1: Prove things about state modification and invariant preservation (not output)*)
 
@@ -14,13 +15,13 @@ Proof.
   2: { intros x. apply prove_st_spec_ret. intros; lia. }
   (*Prove [id_register]*)
   unfold id_register.
-  apply prove_st_spec_bnd_invar with (Q1:=fun i j => i < j)(Q2:=fun i j => i <= j); [| | intros; lia].
-  - (*incr*) apply IdCtr.st_spec_incr. intros.
+  apply prove_st_spec_bnd_invar with (Q1:=fun i j => i <= j)(Q2:=fun i j => i < j); [| | intros; lia].
+  - (*get*) apply IdCtr.st_spec_get. intros; lia.
+  - intros i.
+    apply prove_st_spec_bnd_invar with (Q1:=fun i j => i < j)(Q2:=fun i j => i <= j); [| | intros; lia].
+    + (*incr*) apply IdCtr.st_spec_incr. intros.
     (*TODO: bad*) Transparent CoqBigInt.succ. unfold CoqBigInt.succ. lia. Opaque CoqBigInt.succ.
-  - (*rest of function*) intros _.
-    apply prove_st_spec_bnd_invar with (Q1:=fun i j => i <= j)(Q2:=fun i j => i <= j); [| | intros; lia].
-    + (*get*) apply IdCtr.st_spec_get. intros; lia.
-    + intros x. apply prove_st_spec_ret. intros; lia.
+    + (*rest of function*) intros _. apply prove_st_spec_ret. intros; lia.
 Qed.
 
 Lemma vs_rename_lt m v:
@@ -165,3 +166,657 @@ Proof.
     apply errst_spec_st. eapply st_spec_weaken_post. 2: apply t_open_quant1_lt.
     simpl. destruct (null _); intros; lia.
 Qed.
+
+(*Correctness (only for t_open_bound)*)
+
+(*TODO: move*)
+Lemma errst_spec_tup1 {St1 St2 A: Type} (P1: St1 -> Prop) (Q1: St2 -> Prop) (P2: St1 -> A -> St1 -> Prop) (Q: St2 -> A -> St2 -> Prop) (o: errState St1 A)
+  (*Don't like this but oh well*)
+  (Q_impl: forall s s1 x, Q1 s -> fst (run_errState o s1) = inr x -> Q s x s):
+  errst_spec P1 o P2 ->
+  errst_spec (fun x => P1 (fst x) /\ Q1 (snd x)) (errst_tup1 o) (fun s1 x s2 => P2 (fst s1) x (fst s2) /\ Q (snd s1) x (snd s2)).
+Proof.
+  unfold errst_spec. intros Hspec [i1 i2] b [Hp1 Hq1] Hb.
+  simpl.
+  destruct o; simpl in *. unfold run_errState in *; simpl in *.
+  specialize (Hspec i1).
+  destruct (runState unEitherT i1 ) as [x1 x2] eqn : Hrun; simpl in *; subst.
+  split; auto. eapply Q_impl; auto. rewrite Hrun. auto.
+Qed.
+
+(*TODO*)
+Set Bullet Behavior "Strict Subproofs".
+
+Require Import TermTactics.
+
+Lemma tys_of_term_rewrite t:
+  tys_of_term t =
+  list_of_option_id (t_ty_of t) ++
+  match t_node_of t with
+  | Tvar v => [vs_ty v]
+  | Tconst _ => nil
+  | Tapp l tms => tys_of_lsym l ++ concat (map tys_of_term tms)
+  | Tif t1 t2 t3 => tys_of_term t1 ++ tys_of_term t2 ++ tys_of_term t3
+  | Tlet t1 (v, _, t2) => tys_of_term t1 ++ [vs_ty v] ++ tys_of_term t2
+  | Tcase t ps => tys_of_term t ++ concat (map (fun x => tys_of_pat (fst (fst x)) ++ tys_of_term (snd x)) ps)
+  | Teps (v, _, t) => vs_ty v :: tys_of_term t
+  | Tquant _ (vs, _, _, t) => (map vs_ty vs) ++ tys_of_term t
+  | Tbinop _ t1 t2 => tys_of_term t1 ++ tys_of_term t2
+  | Tnot t => tys_of_term t
+  | _ => nil
+  end.
+Proof.
+  destruct t; simpl. destruct t; reflexivity.
+Qed.
+
+Lemma eqb_eq_reflect {A: Type} {eqb: A -> A -> bool} (eqb_eq: forall x y, x = y <-> eqb x y):
+  forall x y, reflect (x = y) (eqb x y).
+Proof.
+  intros x y. apply iff_reflect. auto.
+Qed.
+
+Lemma oty_equal_spec o1 o2:
+  reflect (o1 = o2) ( oty_equal o1 o2).
+Proof.
+  apply eqb_eq_reflect.
+  apply option_eqb_eq, ty_eqb_eq.
+Qed.
+
+Ltac get_fast_eq :=
+  repeat match goal with
+| H: is_true (term_eqb ?t1 ?t2) |- _ => apply term_eqb_eq in H
+| H: is_true (term_eqb_fast ?t1 ?t2) |- _ => apply term_eqb_eq in H
+| H: is_true (oty_equal ?t1 ?t2) |- _ => destruct (oty_equal_spec t1 t2); [|discriminate]
+| H: is_true (vs_equal ?v1 ?v2) |- _ => apply vsymbol_eqb_eq in H
+| H: is_true (vsymbol_eqb ?v1 ?v2) |- _ => apply vsymbol_eqb_eq in H
+| H: is_true (ls_equal ?l1 ?l2) |- _ => apply lsymbol_eqb_eq in H
+| H: is_true (list_eqb term_eqb_fast ?l1 ?l2) |- _ => apply (list_eqb_eq term_eqb_eq) in H
+| H: is_true (list_eqb term_branch_eqb_fast ?l1 ?l2) |- _ => apply (list_eqb_eq term_branch_eqb_eq) in H
+| H: is_true (list_eqb vsymbol_eqb ?vs1 ?vs2) |- _ => apply (list_eqb_eq vsymbol_eqb_eq) in H
+end.
+
+Ltac solve_similar :=
+  repeat match goal with
+  | x : ?A * ?B |- _ => destruct x
+  end; simpl in *;
+  try rewrite !andb_true in *; destruct_all; get_fast_eq; subst; auto.
+  
+(*Ugh this is really annoying*)
+Lemma t_similar_tys t1 t2:
+  t_similar t1 t2 ->
+  tys_of_term t1 = tys_of_term t2.
+Proof.
+  unfold t_similar. rewrite andb_true.
+  intros [Hoeq Hsim].
+  rewrite !tys_of_term_rewrite.
+  get_fast_eq.
+  rewrite e. f_equal. clear e.
+  destruct_term_node t1; destruct_term_node t2; try discriminate; auto; solve_similar.
+Qed.
+
+Lemma tys_of_term_attr_copy t s:
+  tys_of_term (t_attr_copy t s) = tys_of_term s.
+Proof.
+  unfold t_attr_copy. destruct (t_similar t s && Sattr.is_empty (t_attrs_of s) && negb (isSome (t_loc_of s))) eqn : Hsim.
+  - rewrite !andb_true_iff in Hsim. destruct Hsim as [[Hsim _] _].
+    apply t_similar_tys; auto.
+  - destruct (isNone (t_loc_of s)); simpl; symmetry; rewrite tys_of_term_rewrite at 1; auto.
+Qed.
+
+Print t_map_unsafe.
+
+Lemma t_map_unsafe_rewrite fn t :
+  t_map_unsafe fn t =
+  t_attr_copy t
+  match t_node_of t with
+  | Tapp f tl => t_app1 f (map fn tl) (t_ty_of t)
+  | Tif f t1 t2 => t_if1 (fn f) (fn t1) (fn t2)
+  | Tlet e b => t_let1 (fn e) (bound_map fn b) (t_ty_of t)
+  | Tcase e bl => t_case1 (fn e) (map (bound_map fn) bl) (t_ty_of t)
+  | Teps b => t_eps1 (bound_map fn b) (t_ty_of t)
+  | Tquant q (vl, b, tl, f) => t_quant1 q (vl, b, tr_map fn tl, fn f)
+  | Tbinop op f1 f2 => t_binary1 op (fn f1) (fn f2)
+  | Tnot f1 => t_not1 (fn f1)
+  | _ => t
+  end.
+Proof.
+  reflexivity.
+Qed.
+
+Lemma t_similar_ty t1 t2:
+  t_similar t1 t2 ->
+  t_ty_of t1 = t_ty_of t2.
+Proof.
+  unfold t_similar. rewrite andb_true.
+  intros [Hty _]. get_fast_eq. auto.
+Qed.
+
+Lemma t_attr_copy_ty t s:
+  t_ty_of (t_attr_copy t s) = t_ty_of s.
+Proof.
+  unfold t_attr_copy.
+  destruct (_ && _) eqn : Hsim; auto.
+  bool_hyps. apply t_similar_ty; auto.
+Qed.
+Print term_c.
+(*Need predicate that types are consistent - this is not a full type system*)
+Fixpoint types_wf (t: term_c) : Prop :=
+  match t_node_of t with
+  | Tvar v => t_ty_of t = Some (vs_ty v)
+  | Tconst _ => True
+  | Tapp l tms => (*TODO: need anything else?*)  Forall (fun x => x) (map types_wf tms)
+  | Tif t1 t2 t3 => t_ty_of t2 = t_ty_of t3 /\ t_ty_of t2 = t_ty_of t /\ types_wf t1 /\ types_wf t2 /\ types_wf t3
+  | Tlet t1 (v, _, t2) => (*t_ty_of t1 = Some (vs_ty v) /\ t_ty_of t2 = t_ty_of t /\*) types_wf t1 /\ types_wf t2
+  | Tcase t1 ps => (*TODO: see*) types_wf t1 /\ 
+      Forall (fun x => x) (map (fun x => types_wf (snd x)) ps) (*see if we need more*)
+     (*  Forall (fun x => x) (map (fun x => t_ty_of t1 = Some (pat_ty_of (fst (fst x))) /\
+      t_ty_of (snd x) = t_ty_of t /\ types_wf (snd x)) ps) *)
+  | Teps (v, _, t1) =>  (*t_ty_of t = Some (vs_ty v) /\*) types_wf t1
+  | Tquant _ (vs, _, tr, t1) => t_ty_of t = None /\ types_wf t1
+  | Tbinop _ t1 t2 => t_ty_of t = None /\ (*TODO: do we need to enforce None?*) types_wf t1 /\ types_wf t2
+  | Tnot t1 => t_ty_of t = None /\ types_wf t1
+  | _ => True
+  end.
+
+Lemma types_wf_rewrite t:
+  types_wf t = match t_node_of t with
+  | Tvar v => t_ty_of t = Some (vs_ty v)
+  | Tconst _ => True
+  | Tapp l tms => (*TODO: need anything else?*) Forall (fun x => x) (map types_wf tms)
+  | Tif t1 t2 t3 => t_ty_of t2 = t_ty_of t3 /\ t_ty_of t2 = t_ty_of t /\ types_wf t1 /\ types_wf t2 /\ types_wf t3
+  | Tlet t1 (v, _, t2) => (*t_ty_of t1 = Some (vs_ty v) /\ t_ty_of t2 = t_ty_of t /\*) types_wf t1 /\ types_wf t2
+  | Tcase t1 ps => types_wf t1 /\ 
+      Forall (fun x => x) (map (fun x => types_wf (snd x)) ps)
+  | Teps (v, _, t1) => types_wf t1
+  | Tquant _ (vs, _, tr, t1) => t_ty_of t = None /\ types_wf t1
+  | Tbinop _ t1 t2 => t_ty_of t = None /\ (*TODO: do we need to enforce None?*) types_wf t1 /\ types_wf t2
+  | Tnot t1 => t_ty_of t = None /\ types_wf t1
+  | _ => True
+  end.
+Proof. destruct t; reflexivity.
+Qed.
+
+(*Need wf for var, need this lemma for if below*)
+Lemma ty_subst_unsafe_aux_ty (m: Mvs.t term_c) (t: term_c) (Htywf: types_wf t)
+  (Hvars: forall v t, Mvs.find_opt v m = Some t -> exists v', t = t_var v' /\ vs_ty v = vs_ty v'):
+  (* (Hvars: forall v t, Mvs.find_opt v m = Some t -> t_ty_of t = Some (vs_ty v)): *)
+  t_ty_of (t_subst_unsafe_aux m t) = t_ty_of t.
+Proof.
+  induction t using term_ind_alt; rewrite TermTraverseAux.t_subst_unsafe_aux_rewrite.
+  - (*var*) rewrite Heq, t_attr_copy_ty. rewrite Mvs.find_def_spec.
+    destruct (Mvs.find_opt v m) as [t'|] eqn : Hfind; auto.
+    apply Hvars in Hfind. destruct Hfind as [v' [Ht' Hty]]. subst. simpl.
+    rewrite types_wf_rewrite, Heq in Htywf. congruence.
+  - rewrite Heq, t_map_unsafe_rewrite, Heq, t_attr_copy_ty. reflexivity.
+  - (*app*) rewrite Heq, t_map_unsafe_rewrite, Heq, t_attr_copy_ty. reflexivity.
+  - (*if*) rewrite Heq, t_map_unsafe_rewrite, Heq, t_attr_copy_ty. simpl.
+    (*need wf here*) rewrite types_wf_rewrite, Heq in Htywf. destruct_all.
+    rewrite IHt3; auto. congruence.
+  - (*let*) 
+    rewrite Heq. simpl. rewrite t_attr_copy_ty. simpl. reflexivity.
+  - (*case*) rewrite Heq. simpl. rewrite t_attr_copy_ty. reflexivity.
+  - (*eps*) rewrite Heq. simpl. rewrite t_attr_copy_ty. reflexivity.
+  - (*quant*) rewrite Heq. simpl. rewrite t_attr_copy_ty. simpl. 
+    rewrite types_wf_rewrite, Heq in Htywf. destruct_all; auto.
+  - (*binop*) rewrite Heq, t_map_unsafe_rewrite, Heq, t_attr_copy_ty. simpl.
+    rewrite types_wf_rewrite, Heq in Htywf. destruct_all; auto.
+  - (*not*) rewrite Heq, t_map_unsafe_rewrite, Heq, t_attr_copy_ty. simpl.
+    rewrite types_wf_rewrite, Heq in Htywf. destruct_all; auto.
+  - (*true*) rewrite Ht, t_map_unsafe_rewrite, Ht, t_attr_copy_ty. reflexivity.
+  - (*false*) rewrite Ht, t_map_unsafe_rewrite, Ht, t_attr_copy_ty. reflexivity.
+Qed.
+
+
+(*Any condition of the form: Mvs.find_opt v m = Some t -> P v t holds
+  whenever m shrinks*)
+Check Mvs.t.
+(*TODO: should use this for hash condition*)
+(*m1 \subseteq m2*)
+Definition mvs_submap {A: Type} (m1 m2: Mvs.t A) : Prop :=
+forall x y, Mvs.find_opt x m1 = Some y -> Mvs.find_opt x m2 = Some y.
+
+Lemma mvs_preserved {A: Type} (P: vsymbol -> A -> Prop) 
+  (m1 m2: Mvs.t A) (Hsub: mvs_submap m1 m2) (Hm2: forall v t, Mvs.find_opt v m2 = Some t -> P v t):
+  forall v t, Mvs.find_opt v m1 = Some t -> P v t.
+Proof.
+  intros v t Hfind. apply Hsub in Hfind. auto.
+Qed.
+
+(*For let, eps - *)
+Check Mvs.set_inter.
+Lemma binding_submap {A B: Type} (m: Mvs.t A) (m1: Mvs.t B) (v: vsymbol):
+  mvs_submap (Mvs.set_inter _ _ (Mvs.remove _ v m) m1) m.
+Proof.
+  unfold mvs_submap. intros x y. rewrite Mvs.set_inter_spec.
+  rewrite Mvs.remove_spec. destruct (Vsym.Tg.equal x v); [discriminate|].
+  destruct (Mvs.find_opt x m) eqn : Hopt; auto.
+  destruct (Mvs.find_opt x m1) eqn : Hopt2; auto. discriminate.
+Qed.
+
+Lemma branch_submap {A B C: Type} (m: Mvs.t A) (m1: Mvs.t B) (s: Mvs.t C):
+   mvs_submap (Mvs.set_inter _ _ (Mvs.set_diff _ _ m s) m1) m.
+Proof.
+  unfold mvs_submap. intros x y. rewrite Mvs.set_inter_spec.
+  rewrite Mvs.set_diff_spec.
+  destruct (Mvs.find_opt x m) eqn : Hopt; auto.
+  destruct (Mvs.find_opt x s) eqn : Hopt1; [discriminate|].
+  destruct (Mvs.find_opt x m1) eqn : Hopt2; auto. discriminate.
+Qed.
+
+(*NOTE: maybe separate file with info about [t_subst_unsafe]*)
+Lemma t_subst_unsafe_aux_tys (m: Mvs.t term_c) (t: term_c) (Htywf: types_wf t)
+  (*(Hvars: forall v t, Mvs.find_opt v m = Some t -> t_ty_of t = Some (vs_ty v)):*)
+  (Hvars: forall v t, Mvs.find_opt v m = Some t -> exists v', t = t_var v' /\ vs_ty v = vs_ty v'):
+  (forall x, In x (tys_of_term (t_subst_unsafe_aux m t)) -> In x (tys_of_term t)).
+Proof.
+  intros x. generalize dependent m.
+  induction t using term_ind_alt; intros m Hvars; rewrite TermTraverseAux.t_subst_unsafe_aux_rewrite.
+  - (*var*) rewrite Heq, tys_of_term_attr_copy. rewrite Mvs.find_def_spec.
+    destruct (Mvs.find_opt v m) as [t'|] eqn : Hfind; auto.
+    apply Hvars in Hfind. destruct Hfind as [v' [Ht' Hty]]. subst. simpl.
+    rewrite !tys_of_term_rewrite, Heq, in_app_iff. simpl. 
+    intros; destruct_all; subst; auto; contradiction.
+  - (*const*) rewrite Heq, t_map_unsafe_rewrite, Heq, tys_of_term_attr_copy. auto.
+  - (*app*) rewrite Heq, t_map_unsafe_rewrite, Heq, tys_of_term_attr_copy. simpl.
+    rewrite tys_of_term_rewrite, Heq. rewrite !in_app_iff.
+    rewrite Forall_forall in H. intros [Hin | [Hin | Hin]]; auto.
+    right; right. rewrite in_concat in Hin |- *. destruct Hin as [l1 [Hinl1 Hinx]].
+    rewrite !map_map, in_map_iff in Hinl1. destruct Hinl1 as [tm1 [Hl1 Hint]]; subst.
+    apply H in Hinx; auto.
+    2: { rewrite types_wf_rewrite, Heq, Forall_map, Forall_forall in Htywf. auto. }
+    exists (tys_of_term tm1). split; auto. apply in_map; auto.
+  - (*if*) rewrite Heq, t_map_unsafe_rewrite, Heq, tys_of_term_attr_copy. simpl.
+    rewrite (tys_of_term_rewrite t4), Heq. 
+    rewrite !in_app_iff.
+    rewrite types_wf_rewrite, Heq in Htywf. destruct_all.
+    intros [Hin | [Hin | [Hin | Hin]]].
+    + (*Need previous lemma here*) 
+      rewrite ty_subst_unsafe_aux_ty in Hin; auto.
+      right. right. right. 
+      rewrite tys_of_term_rewrite, in_app_iff. auto.
+    + apply IHt1 in Hin; auto.
+    + apply IHt2 in Hin; auto.
+    + apply IHt3 in Hin; auto.
+  - (*let*) rewrite Heq; simpl. rewrite tys_of_term_attr_copy. simpl.
+    rewrite types_wf_rewrite, Heq in Htywf. destruct_all.
+    rewrite !in_app_iff, (tys_of_term_rewrite t3), Heq, !in_app_iff. simpl.
+    intros [Hin | [Hin | Hin]]; auto.
+    { apply IHt1 in Hin; auto. }
+    destruct Hin as [Hx | Hinx]; auto.
+    destruct (Mvs.is_empty _ _) eqn : Hisemp; auto.
+    apply IHt2 in Hinx; auto.
+    (*Prove condition preserved*)
+    apply mvs_preserved with (m2:=m); auto.
+    apply binding_submap.
+  - (*case*) rewrite Heq; simpl. rewrite tys_of_term_attr_copy. simpl.
+    rewrite (tys_of_term_rewrite t2), Heq, !in_app_iff.
+    rewrite types_wf_rewrite, Heq in Htywf. destruct Htywf as [Hwf1 Hwf2].
+    intros [Hin | [Hin | Hin]]; auto.
+    { apply IHt1 in Hin; auto. }
+    rewrite !map_map in Hin. simpl in Hin.
+    (*Now lots of concat*)
+    right. right. rewrite !in_concat in Hin |- *.
+    destruct Hin as [l1 [Hinl1 Hinx]]. 
+    rewrite in_map_iff in Hinl1. destruct Hinl1 as [pt [Hl1 Hinpt]]; subst.
+    exists (tys_of_pat (fst (fst pt)) ++ tys_of_term (snd pt)).
+    split; [rewrite in_map_iff; exists pt; auto |].
+    rewrite in_app_iff in Hinx |- *. destruct Hinx as [Hinx | Hinx]; auto.
+    destruct (Mvs.is_empty _ _) eqn : Hemp; auto.
+    (*Now use IH, need to get Foralls*)
+    rewrite !Forall_map, !Forall_forall in H, Hwf2.
+    apply H in Hinx; auto.
+    apply mvs_preserved with (m2:=m); auto.
+    apply branch_submap.
+  - (*eps*) rewrite Heq; simpl. rewrite tys_of_term_attr_copy. simpl.
+    rewrite types_wf_rewrite, Heq in Htywf.
+    rewrite (tys_of_term_rewrite t2), Heq, !in_app_iff. simpl.
+    intros [Hin | [Hin | Hin]]; auto.
+    destruct (Mvs.is_empty _ _) eqn : Hisemp; auto.
+    apply IHt1 in Hin; auto.
+    (*Prove condition preserved*)
+    apply mvs_preserved with (m2:=m); auto.
+    apply binding_submap.
+  - (*quant*) rewrite Heq; simpl.  rewrite tys_of_term_attr_copy. simpl.
+    rewrite types_wf_rewrite, Heq in Htywf.
+    rewrite (tys_of_term_rewrite t2), Heq, !in_app_iff. destruct_all.
+    intros [Hin | Hin]; auto. 
+    destruct (Mvs.is_empty _ _) eqn : Hisemp; auto.
+    apply IHt1 in Hin; auto.
+    (*Prove condition preserved*)
+    apply mvs_preserved with (m2:=m); auto.
+    apply branch_submap.
+  - (*binop*) rewrite Heq, t_map_unsafe_rewrite, Heq, tys_of_term_attr_copy. simpl.
+    rewrite types_wf_rewrite, Heq in Htywf. destruct_all. 
+    rewrite (tys_of_term_rewrite t3), Heq, !in_app_iff. 
+    intros [Hin | Hin]; [apply IHt1 in Hin | apply IHt2 in Hin]; auto.
+  - (*not*) rewrite Heq,  t_map_unsafe_rewrite, Heq, tys_of_term_attr_copy. simpl.
+    rewrite types_wf_rewrite, Heq in Htywf. destruct_all. 
+    rewrite (tys_of_term_rewrite t2), Heq, !in_app_iff. intros Hin. apply IHt1 in Hin; auto.
+  - (*true*) rewrite Ht,  t_map_unsafe_rewrite, Ht, tys_of_term_attr_copy. auto.
+  - (*false*) rewrite Ht,  t_map_unsafe_rewrite, Ht, tys_of_term_attr_copy. auto.
+Qed.
+
+Lemma t_subst_unsafe_tys (m: Mvs.t term_c) (t: term_c) (Htywf: types_wf t)
+  (*(Hvars: forall v t, Mvs.find_opt v m = Some t -> t_ty_of t = Some (vs_ty v)):*)
+  (Hvars: forall v t, Mvs.find_opt v m = Some t -> exists v', t = t_var v' /\ vs_ty v = vs_ty v'):
+  (forall x, In x (tys_of_term (t_subst_unsafe m t)) -> In x (tys_of_term t)).
+Proof.
+  intros x. unfold t_subst_unsafe. destruct (Mvs.is_empty term_c m); auto.
+  apply t_subst_unsafe_aux_tys; auto.
+Qed.
+
+Lemma concat_map_sublist {A B: Type} (f: A -> list B) (l1 l2: list A) (Hsub: forall x, In x l1 -> In x l2):
+  forall x, In x (concat (map f l1)) -> In x (concat (map f l2)).
+Proof.
+  intros x Hinx. rewrite in_concat in *. destruct Hinx as [y [Hiny Hinx]]. rewrite in_map_iff in Hiny.
+  destruct Hiny as [z [Hy Hinz]]; subst. exists (f z). split; auto. apply in_map; auto.
+Qed.
+
+(*Prove that [vs_rename] results in variable w correct tag*)
+Lemma rename_tag_spec m v1:
+st_spec (fun _ : CoqWeakhtbl.tag => True) (vs_rename m v1)
+  (fun (s1 : CoqWeakhtbl.tag) (v : Mvs.t term_c * vsymbol) (_ : CoqWeakhtbl.tag) =>
+   id_tag (vs_name (snd v)) = s1).
+Proof.
+  unfold vs_rename.
+  apply prove_st_spec_bnd with (P2:=fun _ _ => True) (Q1:=fun s1 v _ => id_tag (vs_name v) = s1)
+  (Q2:=fun x _ y _ => x = snd y); auto.
+  3: { intros s1 _ _ x y Hid Hx; subst; auto. }
+  2: { intros x. apply prove_st_spec_ret. simpl. auto. }
+  (*TODO: separate lemma for [fresh_vsymbol]?*)
+  unfold fresh_vsymbol, create_vsymbol.
+  eapply prove_st_spec_bnd with (P2:=fun _ _ => True) (Q1:=fun s1 i _ => id_tag i = s1)
+  (Q2:=fun x _ y _ => vs_name y = x); auto.
+  3: { intros s1 _ _ x y Hid Hx; subst; auto. }
+  2: { intros x.  apply prove_st_spec_ret. simpl. auto. }
+  (*id_register part*)
+  unfold id_register. Check prove_st_spec_bnd.
+  apply prove_st_spec_bnd with (P2:=fun s1 i => True) (Q1:=fun s1 i _ => i = s1)
+  (Q2:=fun x _ y _ => id_tag y = x); auto.
+  1: { (*get*) apply IdCtr.st_spec_get. auto. } 
+  2: { intros s1 _ _ x y Hxy; subst; auto. }
+  intros i.
+  (*The rest does not change the output*)
+  eapply prove_st_spec_bnd with (P2:=fun _ _ => True) (Q1:=fun s1 _ _ => True)
+  (Q2:=fun _ _ y _ => id_tag y = i); auto.
+  1: { unfold st_spec; auto. }
+  intros _. apply prove_st_spec_ret. simpl. auto.
+Qed.
+
+
+(*TODO: move maybe*)
+Lemma t_open_bound_var tb1:
+   errst_spec (fun _ => True)
+    (errst_tup1 (errst_lift1 (t_open_bound tb1)))
+  (fun (s1: full_st) (tb2: TermDefs.vsymbol * term_c) s2 => 
+    id_tag (vs_name (fst tb2)) = fst s1).
+Proof.
+  apply errst_spec_weaken_post with (Q1:=fun s1 tb2 _ => id_tag (vs_name (fst tb2)) = fst s1 /\ True);
+  [ intros; tauto|].
+  apply ErrStateHoare.errst_spec_tup1 with (P:=fun s1 tb2 _ => id_tag (vs_name (fst tb2)) = s1) 
+  (Q:=fun _ _ _ => True); auto.
+  apply errst_spec_st.
+  (*main proof*)
+  unfold t_open_bound.
+  destruct tb1 as [[v1 b1] t1].
+  eapply prove_st_spec_bnd with (P1:=fun _ => True) (Q1:=fun s1 v _ => id_tag (vs_name (snd v)) = s1)
+  (P2:=fun _ _ => True) (Q2:=fun x _ y _ => snd x = fst y); auto.
+  3: { intros s1 _ _ x y Hid Hxy; rewrite <- Hxy; auto. }
+  2: { intros [m v]; simpl. apply prove_st_spec_ret. simpl. auto. }
+  apply rename_tag_spec.
+Qed.
+  
+
+(*True of the output of [vs_rename]*)
+(*Just prove full spec*)
+Lemma vs_rename_map m v1:
+  st_spec (fun _ => True) (vs_rename m v1)
+    (fun _ r _ => fst r = Mvs.add v1 (t_var (snd r)) m).
+Proof.
+  unfold vs_rename.
+  eapply prove_st_spec_bnd_nondep with (Q1:=fun _ _ => True) (Q2:= fun _ y _ => fst y = Mvs.add v1 (t_var (snd y)) m); auto.
+  1: { unfold st_spec; auto. }
+  intros x. apply prove_st_spec_ret. auto.
+Qed.
+
+(*So has no idents if empty*)
+(* Lemma vs_rename_map_no_idents v1:
+st_spec (fun _ : CoqWeakhtbl.tag => True) (vs_rename Mvs.empty v1)
+  (fun (_ : CoqWeakhtbl.tag) (r : Mvs.t term_c * vsymbol) (_ : CoqWeakhtbl.tag) => map_no_idents (fst r)).
+Proof.
+  eapply st_spec_weaken_post. 2: apply vs_rename_map.
+  simpl. intros _ x _ Hx. rewrite Hx.
+  unfold map_no_idents. intros y t. rewrite Mvs.add_spec.
+  destruct (Vsym.Tg.equal y v1).
+  - intros Hsome; inversion Hsome; subst; auto. simpl.  *)
+
+(*CANNOT prove no idents*)
+(* Definition map_no_idents (m: Mvs.t term_c) : Prop :=
+  forall x t, Mvs.find_opt x m = Some t -> idents_of_term t = nil. *)
+
+Lemma idents_of_term_rewrite t :
+  idents_of_term t = match t_node_of t with
+  | Tvar v => [vs_name v]
+  | Tapp _ ts => concat (map idents_of_term ts)
+  | Tif t1 t2 t3 => idents_of_term t1 ++ idents_of_term t2 ++ idents_of_term t3
+  | Tlet t1 (v, _, t2) => vs_name v :: idents_of_term t1 ++ idents_of_term t2
+  | Tcase t1 ps =>
+      idents_of_term t1 ++
+      concat
+        (map
+           (fun x : pattern_c * bind_info * term_c =>
+            idents_of_pattern (fst (fst x)) ++ idents_of_term (snd x)) ps)
+  | Teps (v, _, t0) => vs_name v :: idents_of_term t0
+  | Tquant _ (vs, _, _, t0) => map vs_name vs ++ idents_of_term t0
+  | Tbinop _ t1 t2 => idents_of_term t1 ++ idents_of_term t2
+  | Tnot t0 => idents_of_term t0
+  | _ => []
+  end
+.
+Proof.
+destruct t;
+reflexivity.
+Qed.
+
+Definition ident_in_map i (m: Mvs.t term_c) : Prop :=
+  exists x y, Mvs.find_opt x m = Some y /\ In i (idents_of_term y).
+
+Lemma ident_in_submap i (m1 m2: Mvs.t term_c) (Hsub: mvs_submap m1 m2):
+  ident_in_map i m1 ->
+  ident_in_map i m2.
+Proof.
+  unfold ident_in_map, mvs_submap in *.
+  intros [x [y [Hfind Hini]]]. exists x. exists y. split; auto.
+Qed.
+
+
+Lemma similar_idents t s:
+  t_similar t s ->
+  idents_of_term t = idents_of_term s.
+Proof.
+  unfold t_similar. rewrite andb_true.
+  intros [Hoeq Hsim].
+  rewrite !idents_of_term_rewrite.
+  get_fast_eq.
+  (* rewrite e. f_equal. clear e. *)
+  destruct_term_node t; destruct_term_node s; try discriminate; auto; solve_similar.
+Qed.
+
+Lemma t_attr_copy_idents t s: idents_of_term (t_attr_copy t s) = idents_of_term s.
+Proof.
+  unfold t_attr_copy. destruct (t_similar t s && Sattr.is_empty (t_attrs_of s) && negb (isSome (t_loc_of s))) eqn : Hsim; auto.
+  - apply similar_idents. bool_hyps; auto.
+  - rewrite !idents_of_term_rewrite. reflexivity.
+Qed.
+
+Lemma idents_of_subst m t:
+  forall x, In x (idents_of_term (t_subst_unsafe_aux m t)) -> In x (idents_of_term t) \/ ident_in_map x m.
+Proof.
+  intros i. generalize dependent m. induction t using term_ind_alt; intros m; 
+  rewrite TermTraverseAux.t_subst_unsafe_aux_rewrite; try rewrite Heq; try rewrite Ht;
+  try rewrite t_map_unsafe_rewrite; try rewrite Heq; try rewrite Ht; try rewrite t_attr_copy_idents; auto;
+  simpl; try rewrite !in_app_iff; auto.
+  - (*var*) rewrite Mvs.find_def_spec.
+    (* rewrite (idents_of_term_rewrite t), Heq. simpl. 
+     *)
+    destruct (Mvs.find_opt v m) as [v1|] eqn : Hfind; auto.
+    intros Hini. right. unfold ident_in_map. exists v. exists v1. auto.
+  - (*app*) rewrite Forall_forall in H. rewrite map_map, in_concat.
+    intros [l1 [Hinl1 Hini]]. rewrite in_map_iff in Hinl1. destruct Hinl1 as [x [Hl1 Hinx]]. subst.
+    apply H in Hini; auto. destruct Hini; auto. left.
+    rewrite (idents_of_term_rewrite t), Heq. rewrite in_concat. exists (idents_of_term x); split; auto.
+    apply in_map; auto.
+  - (*if*) rewrite (idents_of_term_rewrite t4), Heq, !in_app_iff.
+    intros [Hin | [Hin | Hin]]; [apply IHt1 in Hin | apply IHt2 in Hin | apply IHt3 in Hin]; destruct_all; auto.
+  - (*let*) rewrite (idents_of_term_rewrite t3), Heq; simpl. rewrite in_app_iff.
+    intros [Hi | [Hini | Hini]]; subst; auto.
+    + apply IHt1 in Hini. destruct_all; auto.
+    + destruct (Mvs.is_empty _ _) eqn : Hemp; auto.
+      apply IHt2 in Hini. destruct Hini; auto.
+      right. eapply ident_in_submap; eauto. apply binding_submap.
+  - (*case*) rewrite (idents_of_term_rewrite t2), Heq, in_app_iff. 
+    intros [Hini | Hini].
+    { apply IHt1 in Hini. destruct Hini; auto. }
+    clear -H Hini.
+    rewrite map_map in Hini. simpl in Hini.  
+    rewrite in_concat in Hini. destruct Hini as [l1 [Hinl1 Hini]].
+    rewrite in_map_iff in Hinl1. destruct Hinl1 as [pt [Hl1 Hinpt]]; subst.
+    rewrite in_app_iff in Hini.
+    assert (Himpl: In i (idents_of_pattern (fst (fst pt)) ++ idents_of_term (snd pt)) ->
+      In i (concat (map (fun x => idents_of_pattern (fst (fst x)) ++ idents_of_term (snd x)) tbs))).
+    {
+      rewrite in_concat. intros Hin. exists (idents_of_pattern (fst (fst pt)) ++ idents_of_term (snd pt)).
+      split; auto. rewrite in_map_iff. exists pt; split; auto. } rewrite in_app_iff in Himpl.
+    destruct Hini as [Hini | Hini]; auto.
+    destruct (Mvs.is_empty _ _) eqn : Hemp; auto.
+    rewrite Forall_map, Forall_forall in H. apply H in Hini; auto.
+    destruct Hini; auto.
+    right. eapply ident_in_submap; eauto. apply branch_submap.
+  - (*eps*) rewrite (idents_of_term_rewrite t2), Heq. simpl.
+    intros [Hi | Hini]; auto.
+    destruct (Mvs.is_empty _ _); auto. apply IHt1 in Hini.
+    destruct Hini; auto. right. eapply ident_in_submap; eauto. apply binding_submap.
+  - (*quant*) rewrite (idents_of_term_rewrite t2), Heq, !in_app_iff.
+    intros [Hini | Hini]; auto. destruct (Mvs.is_empty _ _); auto.
+    apply IHt1 in Hini; auto. destruct_all; auto. right.
+    eapply ident_in_submap; eauto. apply branch_submap.
+  - (*binop*) rewrite (idents_of_term_rewrite t3), Heq, in_app_iff. 
+    intros [Hini | Hini]; [apply IHt1 in Hini | apply IHt2 in Hini]; destruct_all; auto.
+  - (*not*) rewrite (idents_of_term_rewrite t2), Heq. auto. 
+Qed.
+
+Definition map_idents_wf (m: Mvs.t term_c) s : Prop :=
+  forall x y, Mvs.find_opt x m = Some y -> idents_of_term_wf y s.
+
+(*Now need to prove this
+  TODO
+*)
+
+(*A corollary of results about maps, ints, and vars*)
+Lemma vs_rename_map_idents_wf v1: st_spec (fun _ : CoqWeakhtbl.tag => True) (vs_rename Mvs.empty v1)
+  (fun (_ : CoqWeakhtbl.tag) (r : Mvs.t term_c * vsymbol) (s2 : CoqWeakhtbl.tag) =>
+   map_idents_wf (fst r) s2).
+Proof.
+  apply st_spec_weaken with (P1:=fun _ => True /\ True /\ True) (Q1:=fun s1 r s2 => id_tag (vs_name (snd r)) = s1 /\ s1 < s2 /\
+    fst r = Mvs.add v1 (t_var (snd r)) Mvs.empty); auto.
+  - (*Prove implication*)
+    intros i x i2 [Hi [Hii2 Hx]]. unfold map_idents_wf.
+    intros x1 y1. rewrite Hx. rewrite Mvs.add_spec, Mvs.empty_spec.
+    destruct (Vsym.Tg.equal x1 v1) eqn : Heq; try discriminate.
+    intros Hsome; inversion Hsome; subst.
+    unfold idents_of_term_wf. simpl. intros i [Hi | []]. subst. auto.
+  - (*spec*)
+    apply st_spec_and; [apply rename_tag_spec |apply st_spec_and; [apply vs_rename_lt| apply vs_rename_map]].
+Qed.
+
+
+(*Then, prove output wf*)
+(*Need that initial vsym is wf for hash pruporses*)
+(*TODO: split pre and post similarly - prove lemma maybe*)
+Lemma t_open_bound_res_wf tb1 (Hwf: types_wf  (snd tb1)) :
+  errst_spec (fun s1 => vsym_st_wf (fst (fst tb1)) s1 /\ term_st_wf (snd tb1) s1)
+    (errst_tup1 (errst_lift1 (t_open_bound tb1)))
+  (fun _ (tb2: TermDefs.vsymbol * term_c) s2 => 
+    vsym_st_wf (fst tb2) s2 /\ term_st_wf (snd tb2) s2).
+Proof.
+  apply errst_spec_weaken with 
+    (P1:=fun s1 => (vsym_ident_wf (fst (fst tb1)) (fst s1) /\
+      idents_of_term_wf (snd tb1) (fst s1)) /\
+      (vsym_hash_wf (fst (fst tb1)) (snd s1) /\ term_hash_wf (snd tb1) (snd s1)))
+    (Q1:=fun _ tb2 s => (vsym_ident_wf (fst tb2) (fst s) /\
+      idents_of_term_wf (snd tb2) (fst s)) /\
+      (vsym_hash_wf (fst tb2) (snd s) /\ term_hash_wf (snd tb2) (snd s))).
+  { intros i. unfold vsym_st_wf, term_st_wf; tauto. }
+  { intros _ x f. unfold vsym_st_wf, term_st_wf; tauto. }
+  eapply errst_spec_tup1 with (P1:=fun s =>  (vsym_ident_wf (fst (fst tb1)) s /\ idents_of_term_wf (snd tb1) s))
+  (Q1:=fun s => vsym_hash_wf (fst (fst tb1)) s /\ term_hash_wf (snd tb1) s)
+  (P2:=fun _ tb2 s => vsym_ident_wf (fst tb2) s /\ idents_of_term_wf (snd tb2) s)
+  (Q:=fun _ tb2 s => vsym_hash_wf (fst tb2) s /\ term_hash_wf (snd tb2) s).
+  - (*Prove hash pres*) intros s x s1.
+    intros [Hhash1 Hhash2].
+    (*Idea: need that this is same vsymbol w diff name*)
+    destruct tb1 as [[v1 b1] t1]. simpl.
+    cbn. (*TODO: bad*) destruct v1 as [vn vty]; simpl in *.
+    destruct (runState (IdCtr.get tt) x). destruct (runState (IdCtr.incr tt) t0). simpl.
+    intros Hinr; inversion Hinr; subst; simpl in *; clear Hinr.
+    split. 
+    + unfold vsym_hash_wf, gen_hash_wf in *. simpl in *. auto.
+    + unfold term_hash_wf, gen_hash_wf in *. simpl in *. destruct Hhash2 as [Hhash2 Hhash3].
+      set (m:=(Mvs.add {| vs_name := vn; vs_ty := vty |}
+                 (t_var
+                    {|
+                      vs_name :=
+                        {|
+                          id_string := id_string vn;
+                          id_attrs := Sattr.union Sattr.empty (id_attrs vn);
+                          id_loc := id_loc vn;
+                          id_tag := CoqWeakhtbl.create_tag t
+                        |};
+                      vs_ty := vty
+                    |}) Mvs.empty)) in *.
+      assert (Hm: forall v t, Mvs.find_opt v m = Some t -> exists v' : vsymbol, t = t_var v' /\ vs_ty v = vs_ty v').
+      {
+        intros v tm1. subst m. rewrite Mvs.add_spec.
+        destruct (Vsym.Tg.equal v {| vs_name := vn; vs_ty := vty |}) eqn : heq.
+        - intros Hsome; inversion Hsome; subst; simpl; auto. apply vsymbol_eqb_eq in heq.
+          subst. eexists. split; [reflexivity | reflexivity].
+        - rewrite Mvs.empty_spec; discriminate.
+      }
+      split.
+      * clear -Hhash2 Hwf Hm. unfold all_in_hashtable in *.
+        intros x Hin. apply concat_map_sublist with (l2:=(tys_of_term t1)) in Hin; auto.
+        apply t_subst_unsafe_tys; auto.
+      * clear -Hhash3 Hwf Hm. unfold all_idents_smaller in *.
+        intros x Hin. apply concat_map_sublist with (l2:=(tys_of_term t1)) in Hin; auto.
+        apply t_subst_unsafe_tys; auto.
+  - (*Now reason about idents*)
+    apply errst_spec_st.
+    unfold t_open_bound.
+    destruct tb1 as [[v1 b1] t1]. simpl.
+    eapply prove_st_spec_bnd_nondep with (Q1:=fun mv s2 => (vsym_ident_wf (snd mv) s2 /\ map_idents_wf (fst mv) s2) /\
+      idents_of_term_wf t1 s2) (Q2:=fun _ vt s2 => vsym_ident_wf (fst vt) s2 /\ idents_of_term_wf (snd vt) s2); auto.
+    + (*Prove rename part - split and use invariant preservation for 2nd*)
+      apply st_spec_and.
+      2: { eapply st_spec_weaken_post with (Q1:=fun s1 _ s2 => idents_of_term_wf t1 s1 /\ s1 < s2).
+        - intros i1 _ i2. unfold idents_of_term_wf. intros [Hall Hi12] i Hi. apply Hall in Hi; lia.
+        - apply st_spec_weaken_pre with (P1:=fun s => idents_of_term_wf t1 s /\ True).
+          + intros; tauto.
+          + apply st_spec_and.
+            * apply st_spec_init.
+            * apply vs_rename_lt.
+      }
+      (*And now prove that new vsym is wf because its value is larger - TODO: should prove
+        that vs_rename results in same val*)
+      apply st_spec_weaken with (P1:=fun _ => True /\ True /\ True) (Q1:=fun s1 v s2 => 
+        id_tag (vs_name (snd v)) = s1 /\ map_idents_wf (fst v) s2 /\ s1 < s2); auto.
+      2: { apply st_spec_and; [apply rename_tag_spec|apply st_spec_and; [apply vs_rename_map_idents_wf | apply vs_rename_lt]]. }
+      intros i x f [Hi [Hwfm Hif]]; subst. split; auto. 
+    + intros [m v]. simpl. apply prove_st_spec_ret. simpl. intros i [[Hv Hmwf] Ht]. split; auto.
+      unfold idents_of_term_wf in *. intros i' Hini'.
+      unfold t_subst_unsafe in Hini'.
+      destruct (Mvs.is_empty _ _); auto. apply idents_of_subst in Hini'.
+      destruct Hini' as [Hin | Hin]; auto.
+      unfold ident_in_map in Hin. unfold map_idents_wf in Hmwf.
+      destruct Hin as [x [y [Hxy Hin]]]. apply Hmwf in Hxy. auto.
+Qed.
+    
