src/proofs/Gen/StateInvarDecompose.v
@@ -10,8 +10,8 @@ Proof.
   intros s.
   unfold term_st_wf, ty_st_wf.
   (*Easier to separate - can we generalize?*)
-  assert (Hidents: idents_of_term_wf t s <-> idents_of_term_wf t1 s /\ idents_of_term_wf t2 s /\
-    idents_of_term_wf t3 s).
+  assert (Hidents: idents_of_term_wf t (fst s) <-> idents_of_term_wf t1 (fst s) /\ idents_of_term_wf t2 (fst s) /\
+    idents_of_term_wf t3 (fst s)).
   {
     destruct_term_node t. inversion Ht; subst. unfold idents_of_term_wf; simpl.
     repeat (setoid_rewrite in_app_iff).
@@ -19,7 +19,8 @@ Proof.
     - intros Hin. split_all; intros i Hini; apply Hin; auto.
     - intros [Hin1 [Hin2 Hin3]] i Hini. destruct_all; eauto.
   }
-  assert (Hhash: term_hash_wf t s <-> term_hash_wf t1 s /\ term_hash_wf t2 s /\ term_hash_wf t3 s /\ ty_hash_wf (t_ty_of t) s).
+  assert (Hhash: term_hash_wf t (snd s) <-> term_hash_wf t1 (snd s) /\ term_hash_wf t2 (snd s) /\ 
+    term_hash_wf t3 (snd s) /\ ty_hash_wf (t_ty_of t) (snd s)).
   {
     unfold term_hash_wf, ty_hash_wf, gen_hash_wf. destruct_term_node t; inversion Ht; subst; simpl.
     rewrite !map_app, !concat_app. unfold all_in_hashtable, all_idents_smaller.
@@ -34,12 +35,12 @@ Qed.
 
 Lemma term_st_wf_let {t t1 tb} (Ht: t_node_of t = TermDefs.Tlet t1 tb):
   forall s,
-  term_st_wf t s <-> term_st_wf t1 s /\ term_st_wf (snd tb) s /\ vsym_st_wf (fst (fst tb)) s /\ ty_hash_wf (t_ty_of t) s.
+  term_st_wf t s <-> term_st_wf t1 s /\ term_st_wf (snd tb) s /\ vsym_st_wf (fst (fst tb)) s /\ ty_hash_wf (t_ty_of t) (snd s).
 Proof.
   intros s. destruct tb as [[v1 b1] t2]. simpl.
   unfold term_st_wf, vsym_st_wf.
-  assert (Hidents: idents_of_term_wf t s <-> idents_of_term_wf t1 s /\ idents_of_term_wf t2 s /\
-    vsym_ident_wf v1 s).
+  assert (Hidents: idents_of_term_wf t (fst s) <-> idents_of_term_wf t1 (fst s) /\ idents_of_term_wf t2 (fst s) /\
+    vsym_ident_wf v1 (fst s)).
   {
     destruct_term_node t. inversion Ht; subst. unfold idents_of_term_wf, vsym_ident_wf; simpl.
     repeat (setoid_rewrite in_app_iff).
@@ -47,7 +48,8 @@ Proof.
     - intros Hin. split_all; auto.
     - intros; destruct_all; eauto.
   }
-  assert (Hhash: term_hash_wf t s <-> term_hash_wf t1 s /\ term_hash_wf t2 s /\ vsym_hash_wf v1 s /\ ty_hash_wf (t_ty_of t) s).
+  assert (Hhash: term_hash_wf t (snd s) <-> term_hash_wf t1 (snd s) /\ term_hash_wf t2 (snd s) /\ vsym_hash_wf v1 (snd s) 
+      /\ ty_hash_wf (t_ty_of t) (snd s)).
   {
     unfold term_hash_wf, ty_hash_wf, vsym_hash_wf, gen_hash_wf. destruct_term_node t; inversion Ht; subst; simpl.
     rewrite !map_app, !concat_app. unfold all_in_hashtable, all_idents_smaller.
